examples/tutorial/Singleton0.v
@@ -1,0 +1,50 @@
+(*** IMP ***)
+
+Require Import Coqlib.
+Require Import ImpPrelude.
+Require Import STS.
+Require Import Behavior.
+Require Import ModSem.
+Require Import Skeleton.
+Require Import PCM.
+Require Import HoareDef.
+
+Set Implicit Arguments.
+
+Section IMP.
+
+  Context `{Σ: GRA.t}.
+  
+  (*
+    *** Exmaple in pseudo-code style ***
+
+        int a = 1;
+        def singleton(): int :=
+            assume(a == 1); // if a <> 1 then the target goes UB
+            a = a - 1;
+            return 1;
+   *)
+
+  Definition singletonF {E} `{callE -< E} `{pE -< E} `{eventE -< E}
+    : list val -> itree E val :=
+    fun args =>
+      _ <- (pargs [] args)?;;
+      a <- trigger PGet;; `a: Z <- a↓?;;
+      assume(a = 1%Z);;;
+      _ <- trigger (PPut (a - 1: Z)%Z↑);;
+      Ret (Vint 1).
+
+  Definition SingletonSem (sk: Sk.t): ModSem.t := {|
+    ModSem.fnsems := [("singleton", cfunU singletonF)];
+    ModSem.mn := "Singleton";
+    ModSem.initial_st := (1: Z)%Z↑;
+  |}
+  .
+
+  Definition Singleton: Mod.t := {|
+    Mod.get_modsem := SingletonSem;
+    Mod.sk := [("singleton", Sk.Gfun)];
+  |}
+  .
+  
+End IMP.
