examples/tutorial/Singleton1.v
@@ -1,0 +1,60 @@
+(*** SPC ***)
+Require Import Coqlib.
+Require Import ImpPrelude.
+Require Import STS.
+Require Import Behavior.
+Require Import ModSem.
+Require Import Skeleton.
+Require Import PCM.
+Require Import HoareDef OpenDef.
+Require Import ProofMode.
+Require Import Singleton0 SingletonRA.
+
+Set Implicit Arguments.
+
+Section SPC.
+
+  Context `{Σ: GRA.t}.
+  Context `{@GRA.inG SingletonRA Σ}.
+
+  (*
+   *** Exmaple in pseudo-code style ***
+
+        def singleton(): int :=
+            return 1;
+   *)
+  
+  Definition singletonA: list val -> itree hEs val :=
+    fun args =>
+      _ <- (pargs [] args)?;;
+      Ret (Vint 1).
+
+  Definition singleton_spec: fspec :=
+    mk_simple (X:=unit)
+      (fun _ =>
+         (ord_top,
+           (fun varg => (⌜varg = ([]: list val)↑⌝ ** (OwnM (Ball)))%I),
+           (fun vret => (⌜vret = (Vint 1)↑⌝)%I)
+      )).
+
+  Definition SingletonSbtb: list (string * fspecbody) :=
+    [("singleton", mk_specbody singleton_spec (cfunU singletonA))].
+
+  Definition SSingletonSem: SModSem.t :=
+    {|
+      SModSem.fnsems := SingletonSbtb;
+      SModSem.mn := "Singleton";
+      SModSem.initial_mr := GRA.embed Ready;
+      SModSem.initial_st := tt↑;
+    |}.
+
+  Definition SSingleton: SMod.t :=
+    {|
+      SMod.get_modsem := fun _ => SSingletonSem;
+      SMod.sk := [("singleton", Sk.Gfun)];
+    |}.
+
+  Variable GlobalStb: Sk.t -> gname -> option fspec.
+  Definition Singleton: Mod.t := (SMod.to_tgt GlobalStb SSingleton).
+
+End SPC.
