examples/tutorial/SingletonRA.v
@@ -1,0 +1,41 @@
+(*** RA ***)
+Require Import Coqlib.
+Require Import ImpPrelude.
+Require Import STS.
+Require Import Behavior.
+Require Import ModSem.
+Require Import Skeleton.
+Require Import PCM.
+Require Import HoareDef.
+Require Import ProofMode.
+Require Import STB.
+
+Set Implicit Arguments.
+
+(* Same RA with Cannon example *)
+Definition SingletonRA: URA.t := Auth.t (Excl.t unit).
+Definition Ready: SingletonRA := Auth.black (M:=(Excl.t _)) (Some tt).
+Definition Ball: SingletonRA := Auth.white (M:=(Excl.t _)) (Some tt).
+Definition Fired: SingletonRA := Auth.excl (M:=(Excl.t _)) (Some tt) (Some tt).
+
+Lemma ReadyBall: Ready ⋅ Ball = Fired.
+Proof.
+  ur. rewrite URA.unit_idl. ss.
+Qed.
+
+Lemma FiredReady: ~ URA.wf (Fired ⋅ Ready).
+Proof.
+  ur. ss.
+Qed.
+
+Lemma FiredBall: ~ URA.wf (Fired ⋅ Ball).
+Proof.
+  ur. ii. des. ur in H. red in H. des. ur in H. destruct ctx; ss.
+Qed.
+
+Lemma BallReady_wf: URA.wf (Ball ⋅ Ready).
+Proof.
+  ur. split.
+  { eexists. rewrite ! URA.unit_id. ss. }
+  { ur. ss. }
+Qed.
