examples/tutorial/SlowAddMain0.v
@@ -1,0 +1,44 @@
+(*** IMP ***)
+Require Import Coqlib.
+Require Import ImpPrelude.
+Require Import STS.
+Require Import Behavior.
+Require Import ModSem.
+Require Import Skeleton.
+Require Import PCM.
+
+
+Set Implicit Arguments.
+
+Section IMP.
+
+  Context `{Σ: GRA.t}.
+
+  (*
+    *** Example in pseudo-code style ***
+
+        def main(): int :=
+            return slow_add(3, 4);
+   *)
+
+  Definition mainF {E} `{callE -< E} `{pE -< E} `{eventE -< E}
+    : list val -> itree E val :=
+    fun args =>
+      _ <- (pargs [] args)?;;
+      `a: val <- ccallU "add" ([Vint 3; Vint 4]);;
+      Ret a.
+
+  Definition MainSem: ModSem.t :=
+    {|
+      ModSem.fnsems := [("main", cfunU mainF)];
+      ModSem.mn := "Main";
+      ModSem.initial_st := tt↑;
+    |}.
+
+  Definition Main: Mod.t :=
+    {|
+      Mod.get_modsem := fun _ => MainSem;
+      Mod.sk := [("main", Sk.Gfun)];
+    |}.
+
+End IMP.
