examples/tutorial/SlowAddMain01proof.v
@@ -1,0 +1,63 @@
+(*** PROOF_IM ***)
+Require Import SlowAddMain0 SlowAddMain1 SlowAdd1 HoareDef SimModSem.
+Require Import Coqlib.
+Require Import ImpPrelude.
+Require Import Skeleton.
+Require Import PCM.
+Require Import ModSem Behavior.
+Require Import Relation_Definitions.
+
+Require Import Relation_Operators.
+Require Import RelationPairs.
+From ITree Require Import
+     Events.MapDefault.
+From ExtLib Require Import
+     Core.RelDec
+     Structures.Maps
+     Data.Map.FMapAList.
+Require Import HTactics ProofMode IPM.
+Require Import OpenDef.
+Require Import STB.
+
+Set Implicit Arguments.
+
+Local Open Scope nat_scope.
+
+Section PRF.
+
+  Context `{Σ: GRA.t}.
+
+  Variable GlobalStb: Sk.t -> gname -> option fspec.
+  
+  Hypothesis GlobalStb_add: forall sk,
+      GlobalStb sk "add" = Some add_spec.
+
+  (* Simple "add" spec for proof *)
+  Definition addSpec (x: Z * Z) := match x with (n, m) => (n + m)%Z end.
+  
+  Let W: Type := Any.t * Any.t.
+
+  Let wf: _ -> W -> Prop :=
+        @mk_wf _ unit
+          (fun _ st_src st_tgt => (⌜st_tgt = tt↑ /\ st_src = (3: Z)%Z↑⌝)%I).
+
+  Theorem correct: refines2 [SlowAddMain0.Main] [SlowAddMain1.Main GlobalStb].
+  Proof.
+    eapply adequacy_local2. econs; ss. i.
+    econstructor 1 with (wf:=wf) (le:=top2); et; ss; cycle 1.
+    { exists tt. red. econs; ss. eapply to_semantic. iIntros "H". iPureIntro. ss. }
+    
+    (* main *)
+    econs; ss.
+    init. harg. mDesAll. des; clarify.
+    unfold mainF, mainM, ccallU.
+    steps. astart 3. acatch; et.
+    hcall (3, 4, addSpec) _ with ""; et.
+    { ss. }
+    steps. astop. mDesAll. des; clarify. steps.
+    hret _; et.
+
+    Unshelve. all: ss. all: try exact 0.
+  Qed.
+  
+End PRF.
