examples/tutorial/SlowAddMain12proof.v
@@ -1,0 +1,71 @@
+(*** PROOF_MA ***)
+Require Import SlowAddMain1 SlowAddMain2 HoareDef SimModSem.
+Require Import Coqlib.
+Require Import ImpPrelude.
+Require Import Skeleton.
+Require Import PCM.
+Require Import ModSem Behavior.
+Require Import Relation_Definitions.
+
+Require Import Relation_Operators.
+Require Import RelationPairs.
+From ITree Require Import
+     Events.MapDefault.
+From ExtLib Require Import
+     Core.RelDec
+     Structures.Maps
+     Data.Map.FMapAList.
+Require Import HTactics HTactics2 ProofMode IPM.
+Require Import OpenDef.
+Require Import STS STB Invariant.
+
+Require Import MapHeader.
+
+Set Implicit Arguments.
+
+Local Open Scope nat_scope.
+
+Section PRF.
+
+  Context `{Σ: GRA.t}.
+
+  Variable GlobalStbM: Sk.t -> gname -> option fspec.
+  Variable GlobalStb: Sk.t -> gname -> option fspec.
+
+  Hypothesis PUREINCL: forall sk, stb_pure_incl (GlobalStbM sk) (GlobalStb sk).
+  
+  Let W: Type := Any.t * Any.t.
+
+  Let wf: _ -> W -> Prop :=
+        @mk_wf _ unit
+          (fun _ st_src st_tgt => (⌜st_src = tt↑ /\ st_tgt = (3: Z)%Z↑⌝)%I).
+
+  Theorem correct: refines2 [SlowAddMain1.Main GlobalStbM] [SlowAddMain2.Main GlobalStb].
+  Proof.
+    eapply adequacy_local2. econs; ss. i.
+    econstructor 1 with (wf:=wf) (le:=top2); et; ss; cycle 1.
+    { exists tt. red. econs; ss. eapply to_semantic. iIntros "H". iFrame. iPureIntro; ss. }
+    
+    (* main *)
+    econs; ss.
+    init. 
+    rename mp_tgt into mpr_tgt.
+    assert(exists mp_src mp_tgt (mr_src mr_tgt: Σ),
+              mrp_src = Any.pair mp_src mr_src↑ ∧ mpr_tgt = Any.pair mp_tgt mr_tgt↑).
+    { inv WF. esplits; et. } des; clarify.
+    harg. fold wf. ss. mDesAll. des; clarify.
+    mAssert (True)%I with "". { ss. }
+    harg_tgt. { iModIntro. iFrame. iSplit; ss. iAssumption. }
+    unfold mainM, mainA, ccallU.
+    steps. hAPC _; et. { iIntros "A". iSplit; et. iAssumption. }
+    steps.
+    hret _; et.
+    { iModIntro. iDestruct "FR" as "[% _]".
+      iPureIntro. split; ss. }
+    { iDestruct "Q" as "[% _]". subst.
+      iPureIntro. rr. esplits; et. }
+
+    Unshelve. all: ss. all: try exact 0.
+  Qed.
+  
+End PRF.
