examples/tutorial/SlowAddMain2.v
@@ -1,0 +1,60 @@
+(*** SPC ***)
+Require Import Coqlib.
+Require Import ImpPrelude.
+Require Import STS.
+Require Import Behavior.
+Require Import ModSem.
+Require Import Skeleton.
+Require Import PCM.
+Require Import HoareDef OpenDef.
+Require Import ProofMode.
+
+Set Implicit Arguments.
+
+Section MID.
+
+  Context `{Σ: GRA.t}.
+
+  (*
+    *** Example in pseudo-code style ***
+
+        def main(): int :=
+            return 7;
+   *)
+  
+  Definition mainA: list val -> itree hEs val :=
+    fun args =>
+      _ <- (pargs [] args)?;;
+      ;;;
+      Ret (Vint 7).
+
+  
+  Definition main_spec: fspec :=
+    mk_simple (X:=unit)
+      (fun _ =>
+         (ord_top,
+           (fun varg => (⌜varg = ([]: list val)↑⌝)%I),
+           (fun vret => (⌜vret = (Vint 7)↑⌝)%I)
+      )).
+  
+  Definition MainSbtbA: list (string * fspecbody) :=
+    [("main", mk_specbody main_spec (cfunU mainA))].
+
+  Definition AMainSem: SModSem.t :=
+    {|
+      SModSem.fnsems := MainSbtbA;
+      SModSem.mn := "Main";
+      SModSem.initial_mr := ε;
+      SModSem.initial_st := tt↑;
+    |}.
+
+  Definition AMain: SMod.t :=
+    {|
+      SMod.get_modsem := fun _ => AMainSem;
+      SMod.sk := [("main", Sk.Gfun)];
+    |}.
+
+  Variable GlobalStb: Sk.t -> gname -> option fspec.
+  Definition Main: Mod.t := (SMod.to_tgt GlobalStb AMain).
+
+End MID.
