examples/tutorial/SlowAddMainproof.v
@@ -1,0 +1,43 @@
+(*** PROOF_IM ***)
+Require Import SlowAddMain0 SlowAddMain2 SlowAdd1 HoareDef SimModSem.
+Require Import SlowAddMain01proof SlowAddMain12proof.
+Require Import Coqlib.
+Require Import ImpPrelude.
+Require Import Skeleton.
+Require Import PCM.
+Require Import ModSem Behavior.
+Require Import Relation_Definitions.
+
+Require Import Relation_Operators.
+Require Import RelationPairs.
+From ITree Require Import
+     Events.MapDefault.
+From ExtLib Require Import
+     Core.RelDec
+     Structures.Maps
+     Data.Map.FMapAList.
+Require Import HTactics ProofMode IPM.
+Require Import OpenDef.
+Require Import STB.
+
+Set Implicit Arguments.
+
+Local Open Scope nat_scope.
+
+Section PRF.
+
+  Context `{Σ: GRA.t}.
+
+  Variable GlobalStb: Sk.t -> gname -> option fspec.
+  
+  Hypothesis GlobalStb_add: forall sk,
+      GlobalStb sk "add" = Some add_spec.
+  
+  Theorem correct: refines2 [SlowAddMain0.Main] [SlowAddMain2.Main GlobalStb].
+  Proof.
+    etrans.
+    { eapply SlowAddMain01proof.correct. apply GlobalStb_add. }
+    { eapply SlowAddMain12proof.correct. i. ss. }
+  Qed.
+
+End PRF.
